rename rel to hrel to avoid clash with rel in MathComp

rel.v
@@ -13,62 +13,62 @@ Require Export boolean prop.
 Require Import kat.
 
 (** a relation between two sets is just a predicate  *)
-Definition rel (n m: Set) := n -> m -> Prop.
+Definition hrel (n m: Set) := n -> m -> Prop.
 
 (** * Relations as a (bounded, distributive) lattice *)
 
 (** lattice operations and laws are obtained for free, by two
    successive pointwise liftings of the [Prop] lattice *)
 
-Canonical Structure rel_lattice_ops n m := 
-  lattice.mk_ops (rel n m) leq weq cup cap neg bot top.
+Canonical Structure hrel_lattice_ops n m := 
+  lattice.mk_ops (hrel n m) leq weq cup cap neg bot top.
 
-Global Instance rel_lattice_laws n m: 
-  lattice.laws (BDL+STR+CNV+DIV) (rel_lattice_ops n m) := pw_laws _. 
+Global Instance hrel_lattice_laws n m: 
+  lattice.laws (BDL+STR+CNV+DIV) (hrel_lattice_ops n m) := pw_laws _. 
 
 (** * Relations as a residuated Kleene allegory *)
 
 (** relational composition *)
-Definition rel_dot n m p (x: rel n m) (y: rel m p): rel n p := 
+Definition hrel_dot n m p (x: hrel n m) (y: hrel m p): hrel n p := 
   fun i j => exists2 k, x i k & y k j.
 
 (** converse (or transpose) *)
-Definition rel_cnv n m (x: rel n m): rel m n := 
+Definition hrel_cnv n m (x: hrel n m): hrel m n := 
   fun i j => x j i.
 
 (** left / right divisions *)
-Definition rel_ldv n m p (x: rel n m) (y: rel n p): rel m p := 
+Definition hrel_ldv n m p (x: hrel n m) (y: hrel n p): hrel m p := 
   fun i j => forall k, x k i -> y k j.
 
-Definition rel_rdv n m p (x: rel m n) (y: rel p n): rel p m := 
+Definition hrel_rdv n m p (x: hrel m n) (y: hrel p n): hrel p m := 
   fun j i => forall k, x i k -> y j k.
 
 Section i.
   Variable n: Set.
-  Variable x: rel n n.
+  Variable x: hrel n n.
   (** finite iterations of a relation *)
-  Fixpoint iter u := match u with O => @eq _ | S u => rel_dot _ _ _ x (iter u) end.
+  Fixpoint iter u := match u with O => @eq _ | S u => hrel_dot _ _ _ x (iter u) end.
   (** Kleene star (reflexive transitive closure) *)
-  Definition rel_str: rel n n := fun i j => exists u, iter u i j.
+  Definition hrel_str: hrel n n := fun i j => exists u, iter u i j.
   (** strict iteration (transitive closure) *)
-  Definition rel_itr: rel n n := rel_dot n n n x rel_str.
+  Definition hrel_itr: hrel n n := hrel_dot n n n x hrel_str.
 End i.
 
 
 (** packing all operations into a monoid; note that the unit on [n] is
    just the equality on [n], i.e., the identity relation on [n] *)
 
-Canonical Structure rel_monoid_ops := 
-  monoid.mk_ops Set rel_lattice_ops rel_dot (@eq) rel_itr rel_str rel_cnv rel_ldv rel_rdv.
+Canonical Structure hrel_monoid_ops := 
+  monoid.mk_ops Set hrel_lattice_ops hrel_dot (@eq) hrel_itr hrel_str hrel_cnv hrel_ldv hrel_rdv.
 
 (** binary relations form a residuated Kleene allegory *)
-Instance rel_monoid_laws: monoid.laws (BDL+STR+CNV+DIV) rel_monoid_ops.
+Instance hrel_monoid_laws: monoid.laws (BDL+STR+CNV+DIV) hrel_monoid_ops.
 Proof.
   assert (dot_leq: forall n m p,
-    Proper (leq ==> leq ==> leq) (rel_dot n m p)).
+    Proper (leq ==> leq ==> leq) (hrel_dot n m p)).
    intros n m p x y H x' y' H' i k [j Hij Hjk]. exists j. apply H, Hij. apply H', Hjk.
   constructor; (try now left); intros. 
-   apply rel_lattice_laws.
+   apply hrel_lattice_laws.
    intros i j. firstorder. 
    intros i j. firstorder congruence.
    intros i j. firstorder. 
@@ -76,9 +76,9 @@ Proof.
    intros x y E i j. apply E.
    intros i j E. exists O. exact E.
    intros i k [j Hij [u Hjk]]. exists (S u). firstorder. 
-   assert (E: forall i, (iter n x i: rel n n) ⋅ z ≦ z).
+   assert (E: forall i, (iter n x i: hrel n n) ⋅ z ≦ z).
     induction i. simpl. firstorder now subst.
-    rewrite <-H0 at 2. transitivity (x⋅((iter n x i: rel n n)⋅z)). 
+    rewrite <-H0 at 2. transitivity (x⋅((iter n x i: hrel n n)⋅z)). 
      simpl. firstorder congruence. now apply dot_leq. 
     intros i j [? [? ?] ?]. eapply E. repeat eexists; eauto.
    reflexivity. 
@@ -93,19 +93,19 @@ Qed.
 (** * Relations as a Kleene algebra with tests *)
 
 (** "decidable" sets or predicates: Boolean functions *)
-Definition dset: ob rel_monoid_ops -> lattice.ops := pw_ops bool_lattice_ops.
+Definition dset: ob hrel_monoid_ops -> lattice.ops := pw_ops bool_lattice_ops.
 
 (** injection of decidable predicates into relations, as sub-identities *)
-Definition rel_inj n (x: dset n): rel n n := fun i j => i=j /\ x i.
+Definition hrel_inj n (x: dset n): hrel n n := fun i j => i=j /\ x i.
 
 (** packing relations and decidable sets as a Kleene algebra with tests *)
-Canonical Structure rel_kat_ops := 
-  kat.mk_ops rel_monoid_ops dset rel_inj.
+Canonical Structure hrel_kat_ops := 
+  kat.mk_ops hrel_monoid_ops dset hrel_inj.
 
-Instance rel_kat_laws: kat.laws rel_kat_ops.
+Instance hrel_kat_laws: kat.laws hrel_kat_ops.
 Proof.
   constructor. apply lower_laws. intro. apply (pw_laws (H:=lower_lattice_laws)).
-  assert (inj_leq: forall n, Proper (leq ==> leq) (@rel_inj n)).
+  assert (inj_leq: forall n, Proper (leq ==> leq) (@hrel_inj n)).
    intros n e f H i j [E H']. split. assumption. revert H'. apply mm_bool_Prop, H.
   constructor; try discriminate. 
   apply inj_leq.
@@ -124,7 +124,7 @@ Qed.
 
 (** * Functional relations  *)
 
-Definition frel {A B: Set} (f: A -> B): rel A B := fun x y => y = f x. 
+Definition frel {A B: Set} (f: A -> B): hrel A B := fun x y => y = f x. 
 
 Lemma frel_comp {A B C: Set} (f: A -> B) (g: B -> C): frel f ⋅ frel g ≡ frel (fun x => g (f x)).
 Proof.
